tests/layeff/LowParseWriters.Parsers.fsti
@@ -1,7 +1,8 @@
 module LowParseWriters.Parsers
 include LowParseWriters
 
-module LP = LowParse.Low
+module LP = LowParse.Low.Base
+module LPI = LowParse.Spec.AllIntegers
 module Seq = FStar.Seq
 module U32 = FStar.UInt32
 
@@ -61,14 +62,6 @@ val size_correct
   (size p x == Seq.length (LP.serialize (get_serializer p) x))
   [SMTPat (size p x)]
 
-val star_correct
-  (p1 p2: parser)
-: Lemma
-  (get_parser_kind (p1 `star` p2) == get_parser_kind p1 `LP.and_then_kind` get_parser_kind p2 /\
-  get_parser (p1 `star` p2) == get_parser p1 `LP.nondep_then` get_parser p2 /\
-  get_serializer (p1 `star` p2) == get_serializer p1 `LP.serialize_nondep_then` get_serializer p2)
-  [SMTPat (p1 `star` p2)]
-
 inline_for_extraction
 val deref
   (#p: parser)
@@ -117,47 +110,21 @@ val valid_synth_parser_eq
   })
 : Tot (valid_synth_t p1 p2 (fun _ -> True) (fun x -> x))
 
-inline_for_extraction
-val parse_synth
-  (p1: parser)
-  (#t2: Type)
-  (f2: dfst p1 -> GTot t2)
-  (f1: t2 -> GTot (dfst p1))
-: Pure parser
-  (requires (
-    LP.synth_injective f2 /\
-    LP.synth_inverse f2 f1
-  ))
-  (ensures (fun r ->
-    LP.synth_injective f2 /\
-    LP.synth_inverse f2 f1 /\
-    dfst r == t2 /\
-    get_parser_kind r == get_parser_kind p1 /\
-    get_parser r == LP.coerce (LP.parser (get_parser_kind r) (dfst r)) (get_parser p1 `LP.parse_synth` f2) /\
-    get_serializer r == LP.coerce (LP.serializer (get_parser r)) (LP.serialize_synth (get_parser p1) f2 (get_serializer p1) f1 ())
-  ))
+let parse_vldata_pred
+  (min: nat)
+  (max: nat)
+  (p: parser)
+  (x: dfst p)
+: GTot Type0
+= let reslen = size p x in
+  min <= reslen /\ reslen <= max
 
-val valid_synth_parse_synth
-  (p1: parser)
-  (#t2: Type)
-  (f2: dfst p1 -> GTot t2)
-  (f1: t2 -> GTot (dfst p1))
-  (sq: squash (
-    LP.synth_injective f2 /\
-    LP.synth_inverse f2 f1
-  ))
-: Tot (valid_synth_t p1 (parse_synth p1 f2 f1) (fun _ -> True) f2)
-
-val valid_synth_parse_synth_recip
-  (p1: parser)
-  (#t2: Type)
-  (f2: dfst p1 -> GTot t2)
-  (f1: t2 -> GTot (dfst p1))
-  (sq: squash (
-    LP.synth_injective f2 /\
-    LP.synth_inverse f2 f1
-  ))
-: Tot (valid_synth_t (parse_synth p1 f2 f1) p1 (fun _ -> True) f1)
+let parse_vldata_t
+  (min: nat)
+  (max: nat)
+  (p: parser)
+: Tot Type
+= (x: dfst p { parse_vldata_pred min max p x } )
 
 inline_for_extraction
 val parse_vldata
@@ -165,11 +132,35 @@ val parse_vldata
   (min: U32.t)
   (max: U32.t { U32.v min <= U32.v max /\ U32.v max > 0 })
 : Tot (p' : parser {
-    dfst p' == LP.parse_bounded_vldata_strong_t (U32.v min) (U32.v max) (get_serializer p) /\
-    get_parser_kind p' == LP.parse_bounded_vldata_strong_kind (U32.v min) (U32.v max) (LP.log256' (U32.v max)) (get_parser_kind p) /\
-    get_parser p' == LP.parse_bounded_vldata_strong (U32.v min) (U32.v max) (get_serializer p) /\
-    get_serializer p' == LP.serialize_bounded_vldata_strong (U32.v min) (U32.v max) (get_serializer p)
+    dfst p' == parse_vldata_t (U32.v min) (U32.v max) p
   })
+
+inline_for_extraction
+let integer_size
+: Type0
+= (y: U32.t { 1 <= U32.v y /\ U32.v y <= 4 })
+
+inline_for_extraction
+let log256
+  (max: U32.t { U32.v max > 0 })
+: Tot integer_size
+=
+  if max `U32.lt` 256ul
+  then 1ul
+  else if max `U32.lt` 65536ul
+  then 2ul
+  else if max `U32.lt` 16777216ul
+  then 3ul
+  else 4ul
+
+val size_parse_vldata
+  (p: parser)
+  (min: U32.t)
+  (max: U32.t { U32.v min <= U32.v max /\ U32.v max > 0 })
+  (x: parse_vldata_t (U32.v min) (U32.v max) p)
+: Lemma
+  (U32.v (log256 max) + size p x == size (parse_vldata p min max) x)
+  [SMTPat (size (parse_vldata p min max) x)]
 
 val valid_synth_parse_vldata
   (p: parser)
@@ -177,24 +168,24 @@ val valid_synth_parse_vldata
   (max: U32.t { U32.v min <= U32.v max /\ U32.v max > 0 })
   (min': U32.t)
   (max': U32.t { U32.v min' <= U32.v max' /\ U32.v max' > 0 })
-: Tot (valid_synth_t (parse_vldata p min max) (parse_vldata p min' max') (fun x -> U32.v min' <= size p x /\ size p x <= U32.v max' /\ LP.log256' (U32.v max') == LP.log256' (U32.v max))
+: Tot (valid_synth_t (parse_vldata p min max) (parse_vldata p min' max') (fun x -> U32.v min' <= size p x /\ size p x <= U32.v max' /\ log256 max == log256 max')
 (fun x -> x))
 
 inline_for_extraction
 val parse_bounded_integer
-  (sz: LP.integer_size)
+  (sz: integer_size)
 : Tot (p' : parser {
-    dfst p' == LP.bounded_integer sz /\
-    get_parser_kind p' == LP.parse_bounded_integer_kind sz /\
-    get_parser p' == LP.parse_bounded_integer sz /\
-    get_serializer p' == LP.serialize_bounded_integer sz
+    dfst p' == LPI.bounded_integer (U32.v sz) /\
+    get_parser_kind p' == LPI.parse_bounded_integer_kind (U32.v sz) /\
+    get_parser p' == LPI.parse_bounded_integer (U32.v sz) /\
+    get_serializer p' == LPI.serialize_bounded_integer (U32.v sz)
   })
 
 let parse_vldata_intro_spec
   (p: parser)
   (min: U32.t)
   (max: U32.t { U32.v min <= U32.v max /\ U32.v max > 0 })
-: Tot (repr_spec unit (parse_bounded_integer (LP.log256' (U32.v max)) `star` p) (parse_vldata p min max) (fun (_, vin) -> U32.v min <= size p vin /\ size p vin <= U32.v max) (fun (_, vin) _ vout -> vin == vout) (fun _ -> False))
+: Tot (repr_spec unit (parse_bounded_integer (log256 max) `star` p) (parse_vldata p min max) (fun (_, vin) -> U32.v min <= size p vin /\ size p vin <= U32.v max) (fun (_, vin) _ vout -> vin == vout) (fun _ -> False))
 =
   fun (_, vin) -> Correct ((), vin)
 
@@ -212,7 +203,7 @@ let parse_vldata_intro
   (p: parser)
   (min: U32.t)
   (max: U32.t { U32.v min <= U32.v max /\ U32.v max > 0 })
-: Write unit (parse_bounded_integer (LP.log256' (U32.v max)) `star` p) (parse_vldata p min max) (fun (_, vin) -> U32.v min <= size p vin /\ size p vin <= U32.v max) (fun (_, vin) _ vout -> vin == vout) inv
+: Write unit (parse_bounded_integer (log256 max) `star` p) (parse_vldata p min max) (fun (_, vin) -> U32.v min <= size p vin /\ size p vin <= U32.v max) (fun (_, vin) _ vout -> vin == vout) inv
 = EWrite?.reflect (| parse_vldata_intro_spec p min max, parse_vldata_intro_impl p min max |)
 
 inline_for_extraction
@@ -222,7 +213,7 @@ let parse_vldata_intro_frame
   (p: parser)
   (min: U32.t)
   (max: U32.t { U32.v min <= U32.v max /\ U32.v max > 0 })
-: Write unit ((frame `star` parse_bounded_integer (LP.log256' (U32.v max))) `star` p) (frame `star` parse_vldata p min max) (fun (_, vin) -> U32.v min <= size p vin /\ size p vin <= U32.v max) (fun ((fr, _), vin) _ (fr', vout) -> fr == fr' /\ (vin <: dfst p) == (vout <: dfst p)) inv
+: Write unit ((frame `star` parse_bounded_integer (log256 (max))) `star` p) (frame `star` parse_vldata p min max) (fun (_, vin) -> U32.v min <= size p vin /\ size p vin <= U32.v max) (fun ((fr, _), vin) _ (fr', vout) -> fr == fr' /\ (vin <: dfst p) == (vout <: dfst p)) inv
 = valid_synth _ _ _ _ _ (valid_synth_star_assoc_1 _ _ _);
   frame2 _ _ _ _ _ _ _ _ (fun _ -> parse_vldata_intro p min max)
 
@@ -230,7 +221,7 @@ let parse_vldata_intro_weak_spec
   (p: parser)
   (min: U32.t)
   (max: U32.t { U32.v min <= U32.v max /\ U32.v max > 0 })
-: Tot (repr_spec unit (parse_bounded_integer (LP.log256' (U32.v max)) `star` p) (parse_vldata p min max) (fun _ -> True) (fun (_, vin) _ vout -> vin == vout) (fun (_, vin) -> ~ (U32.v min <= size p vin /\ size p vin <= U32.v max)))
+: Tot (repr_spec unit (parse_bounded_integer (log256 (max)) `star` p) (parse_vldata p min max) (fun _ -> True) (fun (_, vin) _ vout -> vin == vout) (fun (_, vin) -> ~ (U32.v min <= size p vin /\ size p vin <= U32.v max)))
 =
   fun (_, vin) ->
     let sz = size p vin in
@@ -252,7 +243,7 @@ let parse_vldata_intro_weak
   (p: parser)
   (min: U32.t)
   (max: U32.t { U32.v min <= U32.v max /\ U32.v max > 0 })
-: EWrite unit (parse_bounded_integer (LP.log256' (U32.v max)) `star` p) (parse_vldata p min max) (fun _ -> True) (fun (_, vin) _ vout -> vin == vout) (fun (_, vin) -> ~ (U32.v min <= size p vin /\ size p vin <= U32.v max)) inv
+: EWrite unit (parse_bounded_integer (log256 (max)) `star` p) (parse_vldata p min max) (fun _ -> True) (fun (_, vin) _ vout -> vin == vout) (fun (_, vin) -> ~ (U32.v min <= size p vin /\ size p vin <= U32.v max)) inv
 = EWrite?.reflect (| _, parse_vldata_intro_weak_impl p min max |)
 
 inline_for_extraction
@@ -262,7 +253,7 @@ let parse_vldata_intro_weak_frame
   (p: parser)
   (min: U32.t)
   (max: U32.t { U32.v min <= U32.v max /\ U32.v max > 0 })
-: EWrite unit ((frame `star` parse_bounded_integer (LP.log256' (U32.v max))) `star` p) (frame `star` parse_vldata p min max) (fun _ -> True) (fun ((fr, _), vin) _ (fr', vout) -> fr == fr' /\ (vin <: dfst p) == (vout <: dfst p)) (fun (_, vin) -> ~ (U32.v min <= size p vin /\ size p vin <= U32.v max)) inv
+: EWrite unit ((frame `star` parse_bounded_integer (log256 (max))) `star` p) (frame `star` parse_vldata p min max) (fun _ -> True) (fun ((fr, _), vin) _ (fr', vout) -> fr == fr' /\ (vin <: dfst p) == (vout <: dfst p)) (fun (_, vin) -> ~ (U32.v min <= size p vin /\ size p vin <= U32.v max)) inv
 = 
   valid_synth _ _ _ _ _ (valid_synth_star_assoc_1 _ _ _);
   frame2 _ _ _ _ _ _ _ _ (fun _ -> parse_vldata_intro_weak p min max)
@@ -272,7 +263,7 @@ let parse_vldata_recast_spec
   (min: U32.t)
   (max: U32.t { U32.v min <= U32.v max /\ U32.v max > 0 })
   (min': U32.t)
-  (max': U32.t { U32.v min' <= U32.v max' /\ U32.v max' > 0 /\ LP.log256' (U32.v max) == LP.log256' (U32.v max')})
+  (max': U32.t { U32.v min' <= U32.v max' /\ U32.v max' > 0 /\ log256 (max) == log256 (max')})
 : Tot (repr_spec unit (parse_vldata p min max) (parse_vldata p min' max') (fun _ -> True) (fun vin _ vout -> (vin <: dfst p) == (vout <: dfst p)) (fun vin -> ~ (U32.v min' <= size p vin /\ size p vin <= U32.v max')))
 =
   fun vin ->
@@ -288,7 +279,7 @@ val parse_vldata_recast_impl
   (min: U32.t)
   (max: U32.t { U32.v min <= U32.v max /\ U32.v max > 0 })
   (min': U32.t)
-  (max': U32.t { U32.v min' <= U32.v max' /\ U32.v max' > 0 /\ LP.log256' (U32.v max) == LP.log256' (U32.v max')})
+  (max': U32.t { U32.v min' <= U32.v max' /\ U32.v max' > 0 /\ log256 (max) == log256 (max')})
 : Tot (repr_impl _ _ _ _ _ _ inv (parse_vldata_recast_spec p min max min' max'))
 
 inline_for_extraction
@@ -298,7 +289,7 @@ let parse_vldata_recast
   (min: U32.t)
   (max: U32.t { U32.v min <= U32.v max /\ U32.v max > 0 })
   (min': U32.t)
-  (max': U32.t { U32.v min' <= U32.v max' /\ U32.v max' > 0 /\ LP.log256' (U32.v max) == LP.log256' (U32.v max')})
+  (max': U32.t { U32.v min' <= U32.v max' /\ U32.v max' > 0 /\ log256 (max) == log256 (max')})
 : EWrite unit (parse_vldata p min max) (parse_vldata p min' max') (fun _ -> True) (fun vin _ vout -> (vin <: dfst p) == (vout <: dfst p)) (fun vin -> ~ (U32.v min' <= size p vin /\ size p vin <= U32.v max')) inv
 = EWrite?.reflect (| _, parse_vldata_recast_impl p min max min' max' |)
 
@@ -367,57 +358,24 @@ let rec list_exists
     then true
     else list_exists f_spec f tl
 
-let parse_vllist_t
-  (p: parser1)
-  (min: U32.t)
-  (max: U32.t { U32.v min <= U32.v max /\ U32.v max > 0 })
-: Tot Type
-= let s = LP.serialize_list (get_parser p) (get_serializer p) in
-  LP.parse_bounded_vldata_strong_t (U32.v min) (U32.v max) s
-
-inline_for_extraction
-val parse_vllist
-  (p: parser1)
-  (min: U32.t)
-  (max: U32.t { U32.v min <= U32.v max /\ U32.v max > 0 })
-: Tot (p' : parser {
-    dfst p' == parse_vllist_t p min max /\
-    get_parser_kind p' == LP.parse_bounded_vldata_strong_kind (U32.v min) (U32.v max) (LP.log256' (U32.v max)) LP.parse_list_kind /\
-    get_parser p' == LP.parse_bounded_vldata_strong (U32.v min) (U32.v max) (LP.serialize_list _ (get_serializer p)) /\
-    get_serializer p' == LP.serialize_bounded_vldata_strong (U32.v min) (U32.v max) (LP.serialize_list _ (get_serializer p)) /\
-    True
-  })
-
-inline_for_extraction
-val lptr_of_vllist_ptr
-  (#inv: memory_invariant)
-  (p: parser1)
-  (min: U32.t)
-  (max: U32.t { U32.v min <= U32.v max /\ U32.v max > 0 })
-  (r: ptr (parse_vllist p min max) inv)
-: Read (lptr p inv) True (fun r' -> deref_list_spec r' == (deref_spec r <: list (dfst p))) inv
-
-let list_size
+val list_size
   (p: parser1)
   (x: list (dfst p))
 : GTot nat
-= Seq.length (LP.serialize (LP.serialize_list _ (get_serializer p)) x)
 
-let list_size_nil
+val list_size_nil
   (p: parser1)
 : Lemma
   (list_size p [] == 0)
   [SMTPat (list_size p [])]
-= LP.serialize_list_nil _ (get_serializer p)
 
-let list_size_cons
+val list_size_cons
   (p: parser1)
   (a: dfst p)
   (q: list (dfst p))
 : Lemma
   (list_size p (a :: q) == size p a + list_size p q)
   [SMTPat (list_size p (a :: q))]
-= LP.serialize_list_cons _ (get_serializer p) a q
 
 module L = FStar.List.Tot
 
@@ -431,12 +389,54 @@ let rec list_size_append
   | [] -> ()
   | a :: q -> list_size_append p q l2
 
+let parse_vllist_pred
+  (p: parser1)
+  (min: U32.t)
+  (max: U32.t { U32.v min <= U32.v max /\ U32.v max > 0 })
+  (x: list (dfst p))
+: GTot Type0
+= let s = list_size p x in
+  U32.v min <= s /\ s <= U32.v max
+
+let parse_vllist_t
+  (p: parser1)
+  (min: U32.t)
+  (max: U32.t { U32.v min <= U32.v max /\ U32.v max > 0 })
+: Tot Type
+= (x: list (dfst p) { parse_vllist_pred p min max x })
+
+inline_for_extraction
+val parse_vllist
+  (p: parser1)
+  (min: U32.t)
+  (max: U32.t { U32.v min <= U32.v max /\ U32.v max > 0 })
+: Tot (p' : parser {
+    dfst p' == parse_vllist_t p min max
+  })
+
+val parse_vllist_size
+  (p: parser1)
+  (min: U32.t)
+  (max: U32.t { U32.v min <= U32.v max /\ U32.v max > 0 })
+  (x: parse_vllist_t p min max)
+: Lemma
+  (size (parse_vllist p min max) x == U32.v (log256 max) + list_size p x)
+  [SMTPat (size (parse_vllist p min max) x)]
+
+inline_for_extraction
+val lptr_of_vllist_ptr
+  (#inv: memory_invariant)
+  (p: parser1)
+  (min: U32.t)
+  (max: U32.t { U32.v min <= U32.v max /\ U32.v max > 0 })
+  (r: ptr (parse_vllist p min max) inv)
+: Read (lptr p inv) True (fun r' -> deref_list_spec r' == (deref_spec r <: list (dfst p))) inv
+
 let parse_vllist_nil_spec
   (p: parser1)
   (max: U32.t { U32.v max > 0 })
 : Tot (repr_spec unit emp (parse_vllist p 0ul max) (fun _ -> True) (fun _ _ x -> (x <: list (dfst p)) == [] /\ list_size p x == 0) (fun _ -> False))
 = fun _ ->
-  LP.serialize_list_nil _ (get_serializer p);
   Correct ((), ([] <: parse_vllist_t p 0ul max))
 
 inline_for_extraction
@@ -454,8 +454,6 @@ let parse_vllist_nil
 : Write unit emp (parse_vllist p 0ul max) (fun _ -> True) (fun _ _ x -> (x <: list (dfst p)) == [] /\ list_size p x == 0) inv
 = EWrite?.reflect (| _, parse_vllist_nil_impl p max |)
 
-#push-options "--z3rlimit 32"
-
 let parse_vllist_snoc_spec
   (p: parser1)
   (min: U32.t)
@@ -468,11 +466,7 @@ let parse_vllist_snoc_spec
     (fun _ -> False)
   )
 = fun (l, x) ->
-  LP.serialize_list_singleton _ (get_serializer p) x;
-  LP.serialize_list_append _ (get_serializer p) l [x];
   Correct ((), L.snoc ((l <: list (dfst p)), x))
-
-#pop-options
 
 inline_for_extraction
 val parse_vllist_snoc_impl
@@ -497,8 +491,6 @@ let parse_vllist_snoc
 =
   EWrite?.reflect (| _, parse_vllist_snoc_impl p min max |)
 
-#push-options "--z3rlimit 32"
-
 let parse_vllist_snoc_weak_spec
   (p: parser1)
   (min: U32.t)
@@ -514,13 +506,9 @@ let parse_vllist_snoc_weak_spec
   let sz = list_size p l + size p x in
   if U32.v min <= sz && sz <= U32.v max
   then begin
-    LP.serialize_list_singleton _ (get_serializer p) x;
-    LP.serialize_list_append _ (get_serializer p) l [x];
     Correct ((), L.snoc ((l <: list (dfst p)), x))
   end else
     Error "parse_vllist_snoc_weak: out of bounds"
-
-#pop-options
 
 inline_for_extraction
 val parse_vllist_snoc_weak_impl
@@ -552,7 +540,7 @@ val valid_synth_parse_vllist
   (max: U32.t { U32.v min <= U32.v max /\ U32.v max > 0 })
   (min': U32.t)
   (max': U32.t { U32.v min' <= U32.v max' /\ U32.v max' > 0 })
-: Tot (valid_synth_t (parse_vllist p min max) (parse_vllist p min' max') (fun x -> U32.v min' <= list_size p x /\ list_size p x <= U32.v max' /\ LP.log256' (U32.v max') == LP.log256' (U32.v max))
+: Tot (valid_synth_t (parse_vllist p min max) (parse_vllist p min' max') (fun x -> U32.v min' <= list_size p x /\ list_size p x <= U32.v max' /\ log256 (max) == log256 (max'))
 (fun x -> x))
 
 let parse_vllist_recast_spec
@@ -560,7 +548,7 @@ let parse_vllist_recast_spec
   (min: U32.t)
   (max: U32.t { U32.v min <= U32.v max /\ U32.v max > 0 })
   (min': U32.t)
-  (max': U32.t { U32.v min' <= U32.v max' /\ U32.v max' > 0 /\ LP.log256' (U32.v max) == LP.log256' (U32.v max')})
+  (max': U32.t { U32.v min' <= U32.v max' /\ U32.v max' > 0 /\ log256 max == log256 (max')})
 : Tot (repr_spec unit (parse_vllist p min max) (parse_vllist p min' max') (fun _ -> True) (fun vin _ vout -> (vin <: list (dfst p)) == (vout <: list (dfst p))) (fun vin -> ~ (U32.v min' <= list_size p vin /\ list_size p vin <= U32.v max')))
 =
   fun vin ->
@@ -576,7 +564,7 @@ val parse_vllist_recast_impl
   (min: U32.t)
   (max: U32.t { U32.v min <= U32.v max /\ U32.v max > 0 })
   (min': U32.t)
-  (max': U32.t { U32.v min' <= U32.v max' /\ U32.v max' > 0 /\ LP.log256' (U32.v max) == LP.log256' (U32.v max')})
+  (max': U32.t { U32.v min' <= U32.v max' /\ U32.v max' > 0 /\ log256 (max) == log256 max'})
 : Tot (repr_impl _ _ _ _ _ _ inv (parse_vllist_recast_spec p min max min' max'))
 
 inline_for_extraction
@@ -586,19 +574,30 @@ let parse_vllist_recast
   (min: U32.t)
   (max: U32.t { U32.v min <= U32.v max /\ U32.v max > 0 })
   (min': U32.t)
-  (max': U32.t { U32.v min' <= U32.v max' /\ U32.v max' > 0 /\ LP.log256' (U32.v max) == LP.log256' (U32.v max')})
+  (max': U32.t { U32.v min' <= U32.v max' /\ U32.v max' > 0 /\ log256 (max) == log256 (max')})
 : EWrite unit (parse_vllist p min max) (parse_vllist p min' max') (fun _ -> True) (fun vin _ vout -> (vin <: list (dfst p)) == (vout <: list (dfst p))) (fun vin -> ~ (U32.v min' <= list_size p vin /\ list_size p vin <= U32.v max')) inv
 = EWrite?.reflect (| _, parse_vllist_recast_impl p min max min' max' |)
+
+let parse_vlbytes_pred
+  (min: nat)
+  (max: nat { min <= max /\ max > 0 /\ max < 4294967296 } )
+  (x: FStar.Bytes.bytes)
+: GTot Type0
+= let reslen = FStar.Bytes.length x in
+  min <= reslen /\ reslen <= max
+
+let parse_vlbytes_t
+  (min: nat)
+  (max: nat { min <= max /\ max > 0 /\ max < 4294967296 } )
+: Tot Type
+= (x: FStar.Bytes.bytes { parse_vlbytes_pred min max x } )
 
 inline_for_extraction
 val parse_vlbytes
   (min: U32.t)
   (max: U32.t { U32.v min <= U32.v max /\ U32.v max > 0 })
 : Tot (p' : parser {
-    dfst p' == LP.parse_bounded_vlbytes_t (U32.v min) (U32.v max) /\
-    get_parser_kind p' == LP.parse_bounded_vldata_strong_kind (U32.v min) (U32.v max) (LP.log256' (U32.v max)) LP.parse_all_bytes_kind /\
-    get_parser p' == LP.parse_bounded_vlbytes (U32.v min) (U32.v max) /\
-    get_serializer p' == LP.serialize_bounded_vlbytes (U32.v min) (U32.v max)
+    dfst p' == parse_vlbytes_t (U32.v min) (U32.v max)
   })
 
 module B = LowStar.Buffer
