tests/layeff/LowParseWriters.Compat.fst
@@ -1,0 +1,57 @@
+module LowParseWriters.Compat
+
+friend LowParseWriters.LowParse
+friend LowParseWriters.Parsers
+
+module B = LowStar.Buffer
+
+let star_correct
+  p1 p2
+= ()
+
+let parse_synth
+  p1 #t2 f2 f1
+= make_parser
+    ((dsnd p1).parser `LP.parse_synth` f2)
+    (LP.serialize_synth (dsnd p1).parser f2 (dsnd p1).serializer f1 ())
+    (LP.jump_synth (dsnd p1).jumper f2 ())
+
+let valid_synth_parse_synth
+  p1 #t2 f2 f1 sq
+= {
+  valid_synth_valid = (fun h b pos pos' ->
+    LP.valid_synth h (get_parser p1) f2 (LP.make_slice b (B.len b)) pos
+  );
+  valid_synth_size = (fun x ->
+    LP.synth_injective_synth_inverse_synth_inverse_recip f2 f1 ();
+    LP.serialize_synth_eq (get_parser p1) f2 (dsnd p1).serializer f1 () (f2 x)
+  );
+}
+
+let valid_synth_parse_synth_recip
+  p1 #t2 f2 f1 sq
+= {
+  valid_synth_valid = (fun h b pos pos' ->
+    LP.synth_injective_synth_inverse_synth_inverse_recip f2 f1 ();
+    LP.valid_synth h (get_parser p1) f2 (LP.make_slice b (B.len b)) pos
+  );
+  valid_synth_size = (fun x ->
+    LP.serialize_synth_eq (get_parser p1) f2 (dsnd p1).serializer f1 () (x)
+  );
+}
+
+let parse_vldata_correct
+  p min max
+= ()
+
+let list_size_correct
+  p x
+= ()
+
+let parse_vllist_correct
+  p min max
+= ()
+
+let parse_vlbytes_correct
+  min max
+= ()
