tests/layeff/LowParseWriters.Compat.fsti
@@ -1,0 +1,118 @@
+module LowParseWriters.Compat
+include LowParseWriters.Parsers
+
+module LP = LowParse.Low
+
+val star_correct
+  (p1 p2: parser)
+: Lemma
+  (get_parser_kind (p1 `star` p2) == get_parser_kind p1 `LP.and_then_kind` get_parser_kind p2 /\
+  get_parser (p1 `star` p2) == get_parser p1 `LP.nondep_then` get_parser p2 /\
+  get_serializer (p1 `star` p2) == get_serializer p1 `LP.serialize_nondep_then` get_serializer p2)
+  [SMTPat (p1 `star` p2)]
+
+inline_for_extraction
+val parse_synth
+  (p1: parser)
+  (#t2: Type)
+  (f2: dfst p1 -> GTot t2)
+  (f1: t2 -> GTot (dfst p1))
+: Pure parser
+  (requires (
+    LP.synth_injective f2 /\
+    LP.synth_inverse f2 f1
+  ))
+  (ensures (fun r ->
+    LP.synth_injective f2 /\
+    LP.synth_inverse f2 f1 /\
+    dfst r == t2 /\
+    get_parser_kind r == get_parser_kind p1 /\
+    get_parser r == LP.coerce (LP.parser (get_parser_kind r) (dfst r)) (get_parser p1 `LP.parse_synth` f2) /\
+    get_serializer r == LP.coerce (LP.serializer (get_parser r)) (LP.serialize_synth (get_parser p1) f2 (get_serializer p1) f1 ())
+  ))
+
+val valid_synth_parse_synth
+  (p1: parser)
+  (#t2: Type)
+  (f2: dfst p1 -> GTot t2)
+  (f1: t2 -> GTot (dfst p1))
+  (sq: squash (
+    LP.synth_injective f2 /\
+    LP.synth_inverse f2 f1
+  ))
+: Tot (valid_synth_t p1 (parse_synth p1 f2 f1) (fun _ -> True) f2)
+
+val valid_synth_parse_synth_recip
+  (p1: parser)
+  (#t2: Type)
+  (f2: dfst p1 -> GTot t2)
+  (f1: t2 -> GTot (dfst p1))
+  (sq: squash (
+    LP.synth_injective f2 /\
+    LP.synth_inverse f2 f1
+  ))
+: Tot (valid_synth_t (parse_synth p1 f2 f1) p1 (fun _ -> True) f1)
+
+module U32 = FStar.UInt32
+
+val parse_vldata_correct
+  (p: parser)
+  (min: U32.t)
+  (max: U32.t { U32.v min <= U32.v max /\ U32.v max > 0 })
+: Lemma
+  (
+    let p' = parse_vldata p min max in
+    dfst p' == LP.parse_bounded_vldata_strong_t (U32.v min) (U32.v max) (get_serializer p) /\
+    get_parser_kind p' == LP.parse_bounded_vldata_strong_kind (U32.v min) (U32.v max) (LP.log256' (U32.v max)) (get_parser_kind p) /\
+    get_parser p' == LP.parse_bounded_vldata_strong (U32.v min) (U32.v max) (get_serializer p) /\
+    get_serializer p' == LP.serialize_bounded_vldata_strong (U32.v min) (U32.v max) (get_serializer p)
+  )
+  [SMTPatOr [
+    [SMTPat (dfst (parse_vldata p min max))];
+    [SMTPat (get_parser_kind (parse_vldata p min max))];
+    [SMTPat (get_parser (parse_vldata p min max))];
+    [SMTPat (get_serializer (parse_vldata p min max))];
+  ]]
+
+val list_size_correct
+  (p: parser1)
+  (x: list (dfst p))
+: Lemma
+  (list_size p x == Seq.length (LP.serialize (LP.serialize_list _ (get_serializer p)) x))
+  [SMTPat (list_size p x)]
+
+inline_for_extraction
+val parse_vllist_correct
+  (p: parser1)
+  (min: U32.t)
+  (max: U32.t { U32.v min <= U32.v max /\ U32.v max > 0 })
+: Lemma
+  (let p' = parse_vllist p min max in
+    dfst p' == LP.parse_bounded_vldata_strong_t (U32.v min) (U32.v max) (LP.serialize_list _ (get_serializer p)) /\
+    get_parser_kind p' == LP.parse_bounded_vldata_strong_kind (U32.v min) (U32.v max) (LP.log256' (U32.v max)) LP.parse_list_kind /\
+    get_parser p' == LP.parse_bounded_vldata_strong (U32.v min) (U32.v max) (LP.serialize_list _ (get_serializer p)) /\
+    get_serializer p' == LP.serialize_bounded_vldata_strong (U32.v min) (U32.v max) (LP.serialize_list _ (get_serializer p))
+  )
+  [SMTPatOr [
+    [SMTPat (dfst (parse_vllist p min max))];
+    [SMTPat (get_parser_kind (parse_vllist p min max))];
+    [SMTPat (get_parser (parse_vllist p min max))];
+    [SMTPat (get_serializer (parse_vllist p min max))];
+  ]]
+
+val parse_vlbytes_correct
+  (min: U32.t)
+  (max: U32.t { U32.v min <= U32.v max /\ U32.v max > 0 })
+: Lemma (
+    let p' = parse_vlbytes min max in
+    dfst p' == LP.parse_bounded_vlbytes_t (U32.v min) (U32.v max) /\
+    get_parser_kind p' == LP.parse_bounded_vldata_strong_kind (U32.v min) (U32.v max) (LP.log256' (U32.v max)) LP.parse_all_bytes_kind /\
+    get_parser p' == LP.parse_bounded_vlbytes (U32.v min) (U32.v max) /\
+    get_serializer p' == LP.serialize_bounded_vlbytes (U32.v min) (U32.v max)
+  )
+  [SMTPatOr [
+    [SMTPat (dfst (parse_vlbytes min max))];
+    [SMTPat (get_parser_kind (parse_vlbytes min max))];
+    [SMTPat (get_parser (parse_vlbytes min max))];
+    [SMTPat (get_serializer (parse_vlbytes min max))];
+  ]]
